sync

Qualification/Utils.lean
@@ -2,6 +2,7 @@
 abbrev Rel α β := α → β → Prop
 abbrev EndoRel α := Rel α α
 
+namespace Function
 inductive ReflTransGen {α} (r: EndoRel α): EndoRel α where
   | refl (x: α): ReflTransGen r x x
   | snoc (x y z: α):
@@ -26,9 +27,24 @@ inductive ReflTransLab {State Label: Type} (r: State → Label → State → Pro
       ReflTransLab r s2 l23 s3 →
       ReflTransLab r s1 (l12 :: l23) s3
 
-theorem List.snoc {State Label: Type} {r: State → Label → State → Prop}:
+
+theorem ReflTransLab.snoc {State Label: Type} {r: State → Label → State → Prop}:
   ∀ (s1 s2 s3: State) (l12: List Label) (l23: Label),
       ReflTransLab r s1 l12 s2 →
                    r s2 l23 s3 →
       ReflTransLab r s1 (l23 :: l12) s3
 := by sorry
+
+
+def Function.RelProd {A B C D: Type} (r1: Rel A B) (r2: Rel C D):
+  Rel (A × C) (B × D) :=
+    λ ⟨a,c⟩ ⟨b,d⟩ ↦ r1 a b ∧ r2 c d
+
+
+def Enumeration {α} (P: α → Prop) :=
+  { l: List α // ∀ a, P a ↔ a ∈ l }
+
+example: (λ _:Nat ↦ False).Enumeration :=
+  ⟨[], λ a ↦ by constructor <;> intro h <;> simp at ⊢ h⟩
+
+end Function
